src/impl/TLS13.Impl.Client.Types.fst
@@ -3925,6 +3925,25 @@ let lemma_coalesced_head_step_correct_preserves_end_to_end_invariant
     app_out;
   lemma_client_state_correct_raw_to_message_replay st1
 
+let lemma_coalesced_head_step_correct_preserves_end_to_end_invariant_conditional
+  (st0 st1:CS.connection_state)
+  (resp:client_response)
+  (ev:CS.conn_event)
+  (raw_received:B.bytes)
+  (network_out:B.bytes)
+  (app_out:B.bytes)
+  : Lemma
+      (requires
+        coalesced_head_step_correct
+          st0 st1 resp ev raw_received network_out app_out)
+      (ensures
+        client_end_to_end_invariant st0 ==> client_end_to_end_invariant st1)
+=
+  introduce client_end_to_end_invariant st0 ==> client_end_to_end_invariant st1
+  with
+    lemma_coalesced_head_step_correct_preserves_end_to_end_invariant
+      st0 st1 resp ev raw_received network_out app_out
+
 let coalesced_network_bytes_end_to_end_correct
   (st0 st1:CS.connection_state)
   (buffer_resp:client_buffer_response)
